src/Std/Internal/Do/Triple/SpecLemmas.lean
@@ -31,6 +31,8 @@ import Init.Data.String.Termination
 import Init.Data.String.Lemmas.Iterate
 
 set_option linter.missingDocs true
+-- The `WP`/`WPMonad` split means each lemma uses only the subset of the section variables it needs.
+set_option linter.unusedSectionVars false
 
 @[expose] public section
 
@@ -49,7 +51,7 @@ variable {m : Type u → Type v} {Pred : Type u} {EPred : Type u}
 
 /-! # `Monad` -/
 
-variable [Monad m] [Assertion Pred] [Assertion EPred] [WPMonad m Pred EPred]
+variable [Monad m] [Assertion Pred] [Assertion EPred] [∀ α, WP (m α) α Pred EPred] [WPMonad m Pred EPred]
 
 @[spec]
 theorem Spec.pure (a : α) :
@@ -63,12 +65,12 @@ theorem Spec.bind (x : m α) (f : α → m β) :
     (Triple.iff.mpr PartialOrder.rel_refl) (fun _ => Triple.iff.mpr PartialOrder.rel_refl)
 
 @[spec]
-theorem Spec.map (f : α → β) (x : m α) :
+theorem Spec.map [LawfulMonad m] (f : α → β) (x : m α) :
     Triple (wp x (fun a => post (f a)) epost) (f <$> x) post epost :=
   Triple.map f x (Triple.iff.mpr PartialOrder.rel_refl)
 
 @[spec]
-theorem Spec.seq (x : m (α → β)) (y : m α) :
+theorem Spec.seq [LawfulMonad m] (x : m (α → β)) (y : m α) :
     Triple (wp x (fun f => wp y (fun a => post (f a)) epost) epost) (x <*> y) post epost :=
   Triple.seq x y (Triple.iff.mpr PartialOrder.rel_refl)
 
@@ -88,7 +90,7 @@ theorem Spec.monadLift_ReaderT (x : m α) (post : α → ρ → Pred) :
 
 
 @[spec]
-theorem Spec.monadLift_ExceptT (x : m α) (post : α → Pred) (epost : EPost.Cons (ε → Pred) EPred) :
+theorem Spec.monadLift_ExceptT [LawfulMonad m] (x : m α) (post : α → Pred) (epost : EPost.Cons (ε → Pred) EPred) :
     Triple (wp x post epost.tail) (MonadLift.monadLift x : ExceptT ε m α) post epost :=
   Triple.iff.mpr (WPMonad.le_wp_monadLift_ExceptT_apply x post epost)
 
@@ -156,7 +158,7 @@ theorem Spec.monadMap_refl (x : m α) :
 
 
 @[spec]
-theorem Spec.liftWith_StateT
+theorem Spec.liftWith_StateT [LawfulMonad m]
     (f : (∀{β}, StateT σ m β → m (β × σ)) → m α) (post : α → σ → Pred) :
     Triple (fun s => wp (f (fun x => x.run s)) (fun a => post a s) epost)
       (MonadControl.liftWith (m:=m) f : StateT σ m α) post epost :=
@@ -172,7 +174,7 @@ theorem Spec.liftWith_ReaderT
 
 
 @[spec]
-theorem Spec.liftWith_ExceptT
+theorem Spec.liftWith_ExceptT [LawfulMonad m]
     (f : (∀{β}, ExceptT ε m β → m (Except ε β)) → m α) (post : α → Pred) (epost : EPost.Cons (ε → Pred) EPred) :
     Triple (wp (f (fun x => x.run)) post epost.tail)
       (MonadControl.liftWith (m:=m) f : ExceptT ε m α) post epost :=
@@ -283,25 +285,25 @@ theorem Spec.modifyGet_StateT (f : σ → α × σ) (post : α → σ → Pred) 
 
 /-! # Lifting `MonadStateOf` -/
 
-omit [Monad m] [Assertion Pred] [Assertion EPred] [WPMonad m Pred EPred] in
+omit [Monad m] [Assertion Pred] [Assertion EPred] [∀ α, WP (m α) α Pred EPred] [WPMonad m Pred EPred] in
 theorem Spec.UnfoldLift.get [MonadLift m n] [MonadStateOf σ m] :
     (MonadStateOf.get : n σ) = monadLift (MonadStateOf.get : m σ) := rfl
 
-omit [Monad m] [Assertion Pred] [Assertion EPred] [WPMonad m Pred EPred] in
+omit [Monad m] [Assertion Pred] [Assertion EPred] [∀ α, WP (m α) α Pred EPred] [WPMonad m Pred EPred] in
 theorem Spec.UnfoldLift.set [MonadLift m n] [MonadStateOf σ m] (s : σ) :
     (MonadStateOf.set (m := n) s) = monadLift (MonadStateOf.set (m := m) s) := rfl
 
-omit [Monad m] [Assertion Pred] [Assertion EPred] [WPMonad m Pred EPred] in
+omit [Monad m] [Assertion Pred] [Assertion EPred] [∀ α, WP (m α) α Pred EPred] [WPMonad m Pred EPred] in
 theorem Spec.UnfoldLift.modifyGet [MonadLift m n] [MonadStateOf σ m] (f : σ → α × σ) :
     MonadStateOf.modifyGet (m := n) f = monadLift (MonadStateOf.modifyGet (m := m) f) := rfl
 
 /-! # Lifting `MonadReaderOf` -/
 
-omit [Monad m] [Assertion Pred] [Assertion EPred] [WPMonad m Pred EPred] in
+omit [Monad m] [Assertion Pred] [Assertion EPred] [∀ α, WP (m α) α Pred EPred] [WPMonad m Pred EPred] in
 theorem Spec.UnfoldLift.read [MonadLift m n] [MonadReaderOf ρ m] :
     (MonadReaderOf.read : n ρ) = monadLift (MonadReaderOf.read : m ρ) := rfl
 
-omit [Monad m] [Assertion Pred] [Assertion EPred] [WPMonad m Pred EPred] in
+omit [Monad m] [Assertion Pred] [Assertion EPred] [∀ α, WP (m α) α Pred EPred] [WPMonad m Pred EPred] in
 theorem Spec.UnfoldLift.withReader [MonadFunctor m n] [MonadWithReaderOf ρ m] (f : ρ → ρ) :
     (MonadWithReaderOf.withReader f : n α → n α) = monadMap (m := m) (MonadWithReaderOf.withReader f) := rfl
 
@@ -327,21 +329,21 @@ theorem Spec.throw_ExceptT (err : ε) (post : α → Pred) (epost : EPost.Cons (
 
 
 @[spec]
-theorem Spec.tryCatch_ExceptT (x : ExceptT ε m α) (h : ε → ExceptT ε m α) (post : α → Pred) (epost : EPost.Cons (ε → Pred) EPred) :
+theorem Spec.tryCatch_ExceptT [LawfulMonad m] (x : ExceptT ε m α) (h : ε → ExceptT ε m α) (post : α → Pred) (epost : EPost.Cons (ε → Pred) EPred) :
     Triple (wp x post ⟨fun e => wp (h e) post epost, epost.tail⟩)
       (MonadExceptOf.tryCatch x h : ExceptT ε m α) post epost :=
   Triple.iff.mpr (WPMonad.le_wp_tryCatch_ExceptT_apply x h)
 
 
 @[spec]
-theorem Spec.orElse_ExceptT (x : ExceptT ε m α) (h : Unit → ExceptT ε m α) (post : α → Pred) (epost : EPost.Cons (ε → Pred) EPred) :
+theorem Spec.orElse_ExceptT [LawfulMonad m] (x : ExceptT ε m α) (h : Unit → ExceptT ε m α) (post : α → Pred) (epost : EPost.Cons (ε → Pred) EPred) :
     Triple (wp x post ⟨fun _ => wp (h ()) post epost, epost.tail⟩)
       (OrElse.orElse x h : ExceptT ε m α) post epost :=
   Triple.iff.mpr (WPMonad.le_wp_orElse_ExceptT_apply x h)
 
 
 @[spec]
-theorem Spec.adapt_ExceptT (f : ε → ε') (x : ExceptT ε m α) (post : α → Pred) (epost : EPost.Cons (ε' → Pred) EPred) :
+theorem Spec.adapt_ExceptT [LawfulMonad m] (f : ε → ε') (x : ExceptT ε m α) (post : α → Pred) (epost : EPost.Cons (ε' → Pred) EPred) :
     Triple (wp x post ⟨fun e => epost.head (f e), epost.tail⟩)
       (ExceptT.adapt f x : ExceptT ε' m α) post epost :=
   Triple.iff.mpr (WPMonad.le_wp_adapt_ExceptT_apply f x)
@@ -366,7 +368,7 @@ theorem Spec.tryCatch_Except (x : Except ε α) (h : ε → Except ε α) :
 theorem Spec.orElse_Except (x : Except ε α) (h : Unit → Except ε α) :
     Triple (wp x post epost⟨fun (_ : ε) => wp (h ()) post epost⟩)
       (OrElse.orElse x h : Except ε α) post epost :=
-  Triple.iff.mpr (by simp only [wp, WPMonad.wpTrans, OrElse.orElse, MonadExcept.orElse]; cases x <;> rfl)
+  Triple.iff.mpr (by simp only [wp, WP.wpTrans, OrElse.orElse, MonadExcept.orElse]; cases x <;> rfl)
 
 /-! # `OptionT` -/
 
@@ -509,7 +511,7 @@ theorem Spec.throw_ExceptT_lift [MonadExceptOf ε m] (err : ε) (post : α → P
     Triple (wp (MonadExceptOf.throw (ε:=ε) err : m (@Except.{u, u} ε' α))
         (fun r => match r with | .ok a => post a | .error e => epost.head e) epost.tail)
       (MonadExceptOf.throw (ε:=ε) err : ExceptT ε' m α) post epost :=
-  Triple.iff.mpr (by rw [WPMonad.wp_throw_lift_ExceptT_apply_eq]; apply WPMonad.wp_consequence; intro r; cases r <;> rfl)
+  Triple.iff.mpr (by rw [WPMonad.wp_throw_lift_ExceptT_apply_eq]; apply WP.wp_consequence; intro r; cases r <;> rfl)
 
 
 @[spec]
@@ -544,7 +546,7 @@ theorem Spec.tryCatch_ExceptT_lift [MonadExceptOf ε m] (x : ExceptT ε' m α) (
     Triple (wp (MonadExceptOf.tryCatch (ε:=ε) x h : m (@Except.{u, u} ε' α))
         (fun | .ok a => post a | .error e => epost.head e) epost.tail)
       (MonadExceptOf.tryCatch (ε:=ε) x h : ExceptT ε' m α) post epost :=
-  Triple.iff.mpr (by rw [WPMonad.wp_tryCatch_lift_ExceptT_apply_eq]; apply WPMonad.wp_consequence; intro r; cases r <;> rfl)
+  Triple.iff.mpr (by rw [WPMonad.wp_tryCatch_lift_ExceptT_apply_eq]; apply WP.wp_consequence; intro r; cases r <;> rfl)
 
 
 @[spec]
@@ -601,7 +603,7 @@ open Lean.Order
 universe u₁ u₂ v
 
 variable {α : Type u₁} {β : Type (max u₁ u₂)} {m : Type (max u₁ u₂) → Type v} {Pred : Type (max u₁ u₂)} {EPred : Type (max u₁ u₂)}
-variable [Monad m] [Assertion Pred] [Assertion EPred] [WPMonad m Pred EPred]
+variable [Monad m] [Assertion Pred] [Assertion EPred] [∀ α, WP (m α) α Pred EPred] [WPMonad m Pred EPred]
 
 /-- The type of loop invariants used by the specifications of `for ... in ...` loops.
 A loop invariant maps the iteration cursor and accumulator state to an assertion.
@@ -760,7 +762,7 @@ theorem Spec.foldlM_list_const_inv [LawfulMonad m]
 
 @[spec]
 theorem Spec.forIn'_range {β : Type u} {m : Type u → Type v} {Pred : Type u} {EPred : Type u}
-    [Monad m] [Assertion Pred] [Assertion EPred] [WPMonad m Pred EPred]
+    [Monad m] [Assertion Pred] [Assertion EPred] [∀ α, WP (m α) α Pred EPred] [WPMonad m Pred EPred]
     {xs : Std.Legacy.Range} {init : β} {f : (a : Nat) → a ∈ xs → β → m (ForInStep β)}
     (inv : Invariant xs.toList β Pred)
     {epost : EPred}
@@ -783,7 +785,7 @@ theorem Spec.forIn'_range {β : Type u} {m : Type u → Type v} {Pred : Type u} 
 
 @[spec]
 theorem Spec.forIn_range {β : Type u} {m : Type u → Type v} {Pred : Type u} {EPred : Type u}
-    [Monad m] [Assertion Pred] [Assertion EPred] [WPMonad m Pred EPred]
+    [Monad m] [Assertion Pred] [Assertion EPred] [∀ α, WP (m α) α Pred EPred] [WPMonad m Pred EPred]
     {xs : Std.Legacy.Range} {init : β} {f : Nat → β → m (ForInStep β)}
     (inv : Invariant xs.toList β Pred)
     {epost : EPred}
@@ -807,7 +809,7 @@ open Std Std.PRange in
 
 @[spec]
 theorem Spec.forIn'_rcc {α β : Type u} {m : Type u → Type v} {Pred : Type u} {EPred : Type u}
-    [Monad m] [Assertion Pred] [Assertion EPred] [WPMonad m Pred EPred] [LawfulMonad m]
+    [Monad m] [Assertion Pred] [Assertion EPred] [∀ α, WP (m α) α Pred EPred] [WPMonad m Pred EPred] [LawfulMonad m]
     [LE α] [DecidableLE α] [UpwardEnumerable α] [Rxc.IsAlwaysFinite α]
     [LawfulUpwardEnumerable α] [LawfulUpwardEnumerableLE α]
     {xs : Rcc α} {init : β} {f : (a : α) → a ∈ xs → β → m (ForInStep β)}
@@ -833,7 +835,7 @@ open Std Std.PRange in
 
 @[spec]
 theorem Spec.forIn_rcc {α β : Type u} {m : Type u → Type v} {Pred : Type u} {EPred : Type u}
-    [Monad m] [Assertion Pred] [Assertion EPred] [WPMonad m Pred EPred] [LawfulMonad m]
+    [Monad m] [Assertion Pred] [Assertion EPred] [∀ α, WP (m α) α Pred EPred] [WPMonad m Pred EPred] [LawfulMonad m]
     [LE α] [DecidableLE α] [UpwardEnumerable α] [Rxc.IsAlwaysFinite α]
     [LawfulUpwardEnumerable α] [LawfulUpwardEnumerableLE α]
     {xs : Rcc α} {init : β} {f : α → β → m (ForInStep β)}
@@ -859,7 +861,7 @@ open Std Std.PRange in
 
 @[spec]
 theorem Spec.forIn'_rco {α β : Type u} {m : Type u → Type v} {Pred : Type u} {EPred : Type u}
-    [Monad m] [Assertion Pred] [Assertion EPred] [WPMonad m Pred EPred] [LawfulMonad m]
+    [Monad m] [Assertion Pred] [Assertion EPred] [∀ α, WP (m α) α Pred EPred] [WPMonad m Pred EPred] [LawfulMonad m]
     [LE α] [LT α] [DecidableLT α] [UpwardEnumerable α] [Rxo.IsAlwaysFinite α]
     [LawfulUpwardEnumerable α] [LawfulUpwardEnumerableLE α] [LawfulUpwardEnumerableLT α]
     {xs : Rco α} {init : β} {f : (a : α) → a ∈ xs → β → m (ForInStep β)}
@@ -885,7 +887,7 @@ open Std Std.PRange in
 
 @[spec]
 theorem Spec.forIn_rco {α β : Type u} {m : Type u → Type v} {Pred : Type u} {EPred : Type u}
-    [Monad m] [Assertion Pred] [Assertion EPred] [WPMonad m Pred EPred] [LawfulMonad m]
+    [Monad m] [Assertion Pred] [Assertion EPred] [∀ α, WP (m α) α Pred EPred] [WPMonad m Pred EPred] [LawfulMonad m]
     [LE α] [LT α] [DecidableLT α] [UpwardEnumerable α] [Rxo.IsAlwaysFinite α]
     [LawfulUpwardEnumerable α] [LawfulUpwardEnumerableLE α] [LawfulUpwardEnumerableLT α]
     {xs : Rco α} {init : β} {f : α → β → m (ForInStep β)}
@@ -911,7 +913,7 @@ open Std Std.PRange in
 
 @[spec]
 theorem Spec.forIn'_rci {α β : Type u} {m : Type u → Type v} {Pred : Type u} {EPred : Type u}
-    [Monad m] [Assertion Pred] [Assertion EPred] [WPMonad m Pred EPred] [LawfulMonad m]
+    [Monad m] [Assertion Pred] [Assertion EPred] [∀ α, WP (m α) α Pred EPred] [WPMonad m Pred EPred] [LawfulMonad m]
     [LE α] [UpwardEnumerable α] [Rxi.IsAlwaysFinite α]
     [LawfulUpwardEnumerable α] [LawfulUpwardEnumerableLE α]
     {xs : Rci α} {init : β} {f : (a : α) → a ∈ xs → β → m (ForInStep β)}
@@ -937,7 +939,7 @@ open Std Std.PRange in
 
 @[spec]
 theorem Spec.forIn_rci {α β : Type u} {m : Type u → Type v} {Pred : Type u} {EPred : Type u}
-    [Monad m] [Assertion Pred] [Assertion EPred] [WPMonad m Pred EPred] [LawfulMonad m]
+    [Monad m] [Assertion Pred] [Assertion EPred] [∀ α, WP (m α) α Pred EPred] [WPMonad m Pred EPred] [LawfulMonad m]
     [LE α] [UpwardEnumerable α] [Rxi.IsAlwaysFinite α]
     [LawfulUpwardEnumerable α] [LawfulUpwardEnumerableLE α]
     {xs : Rci α} {init : β} {f : α → β → m (ForInStep β)}
@@ -963,7 +965,7 @@ open Std Std.PRange in
 
 @[spec]
 theorem Spec.forIn'_roc {α β : Type u} {m : Type u → Type v} {Pred : Type u} {EPred : Type u}
-    [Monad m] [Assertion Pred] [Assertion EPred] [WPMonad m Pred EPred] [LawfulMonad m]
+    [Monad m] [Assertion Pred] [Assertion EPred] [∀ α, WP (m α) α Pred EPred] [WPMonad m Pred EPred] [LawfulMonad m]
     [LE α] [DecidableLE α] [LT α] [UpwardEnumerable α] [Rxc.IsAlwaysFinite α]
     [LawfulUpwardEnumerable α] [LawfulUpwardEnumerableLE α] [LawfulUpwardEnumerableLT α]
     {xs : Roc α} {init : β} {f : (a : α) → a ∈ xs → β → m (ForInStep β)}
@@ -988,7 +990,7 @@ theorem Spec.forIn'_roc {α β : Type u} {m : Type u → Type v} {Pred : Type u}
 open Std Std.PRange in
 
 theorem Spec.forIn_roc {α β : Type u} {m : Type u → Type v} {Pred : Type u} {EPred : Type u}
-    [Monad m] [Assertion Pred] [Assertion EPred] [WPMonad m Pred EPred] [LawfulMonad m]
+    [Monad m] [Assertion Pred] [Assertion EPred] [∀ α, WP (m α) α Pred EPred] [WPMonad m Pred EPred] [LawfulMonad m]
     [LE α] [DecidableLE α] [LT α] [UpwardEnumerable α] [Rxc.IsAlwaysFinite α]
     [LawfulUpwardEnumerable α] [LawfulUpwardEnumerableLE α] [LawfulUpwardEnumerableLT α]
     {xs : Roc α} {init : β} {f : α → β → m (ForInStep β)}
@@ -1014,7 +1016,7 @@ open Std Std.PRange in
 
 @[spec]
 theorem Spec.forIn'_roo {α β : Type u} {m : Type u → Type v} {Pred : Type u} {EPred : Type u}
-    [Monad m] [Assertion Pred] [Assertion EPred] [WPMonad m Pred EPred] [LawfulMonad m]
+    [Monad m] [Assertion Pred] [Assertion EPred] [∀ α, WP (m α) α Pred EPred] [WPMonad m Pred EPred] [LawfulMonad m]
     [LT α] [DecidableLT α] [UpwardEnumerable α] [Rxo.IsAlwaysFinite α]
     [LawfulUpwardEnumerable α] [LawfulUpwardEnumerableLT α]
     {xs : Roo α} {init : β} {f : (a : α) → a ∈ xs → β → m (ForInStep β)}
@@ -1040,7 +1042,7 @@ open Std Std.PRange in
 
 @[spec]
 theorem Spec.forIn_roo {α β : Type u} {m : Type u → Type v} {Pred : Type u} {EPred : Type u}
-    [Monad m] [Assertion Pred] [Assertion EPred] [WPMonad m Pred EPred] [LawfulMonad m]
+    [Monad m] [Assertion Pred] [Assertion EPred] [∀ α, WP (m α) α Pred EPred] [WPMonad m Pred EPred] [LawfulMonad m]
     [LT α] [DecidableLT α] [UpwardEnumerable α] [Rxo.IsAlwaysFinite α]
     [LawfulUpwardEnumerable α] [LawfulUpwardEnumerableLT α]
     {xs : Roo α} {init : β} {f : α → β → m (ForInStep β)}
@@ -1066,7 +1068,7 @@ open Std Std.PRange in
 
 @[spec]
 theorem Spec.forIn'_roi {α β : Type u} {m : Type u → Type v} {Pred : Type u} {EPred : Type u}
-    [Monad m] [Assertion Pred] [Assertion EPred] [WPMonad m Pred EPred] [LawfulMonad m]
+    [Monad m] [Assertion Pred] [Assertion EPred] [∀ α, WP (m α) α Pred EPred] [WPMonad m Pred EPred] [LawfulMonad m]
     [LT α] [DecidableLT α] [UpwardEnumerable α] [Rxi.IsAlwaysFinite α]
     [LawfulUpwardEnumerable α] [LawfulUpwardEnumerableLT α]
     {xs : Roi α} {init : β} {f : (a : α) → a ∈ xs → β → m (ForInStep β)}
@@ -1092,7 +1094,7 @@ open Std Std.PRange in
 
 @[spec]
 theorem Spec.forIn_roi {α β : Type u} {m : Type u → Type v} {Pred : Type u} {EPred : Type u}
-    [Monad m] [Assertion Pred] [Assertion EPred] [WPMonad m Pred EPred] [LawfulMonad m]
+    [Monad m] [Assertion Pred] [Assertion EPred] [∀ α, WP (m α) α Pred EPred] [WPMonad m Pred EPred] [LawfulMonad m]
     [LT α] [DecidableLT α] [UpwardEnumerable α] [Rxi.IsAlwaysFinite α]
     [LawfulUpwardEnumerable α] [LawfulUpwardEnumerableLT α]
     {xs : Roi α} {init : β} {f : α → β → m (ForInStep β)}
@@ -1118,7 +1120,7 @@ open Std Std.PRange in
 
 @[spec]
 theorem Spec.forIn'_ric {α β : Type u} {m : Type u → Type v} {Pred : Type u} {EPred : Type u}
-    [Monad m] [Assertion Pred] [Assertion EPred] [WPMonad m Pred EPred] [LawfulMonad m]
+    [Monad m] [Assertion Pred] [Assertion EPred] [∀ α, WP (m α) α Pred EPred] [WPMonad m Pred EPred] [LawfulMonad m]
     [Least? α] [LE α] [DecidableLE α] [UpwardEnumerable α] [Rxc.IsAlwaysFinite α]
     [LawfulUpwardEnumerable α] [LawfulUpwardEnumerableLeast? α] [LawfulUpwardEnumerableLE α]
     {xs : Ric α} {init : β} {f : (a : α) → a ∈ xs → β → m (ForInStep β)}
@@ -1144,7 +1146,7 @@ open Std Std.PRange in
 
 @[spec]
 theorem Spec.forIn_ric {α β : Type u} {m : Type u → Type v} {Pred : Type u} {EPred : Type u}
-    [Monad m] [Assertion Pred] [Assertion EPred] [WPMonad m Pred EPred] [LawfulMonad m]
+    [Monad m] [Assertion Pred] [Assertion EPred] [∀ α, WP (m α) α Pred EPred] [WPMonad m Pred EPred] [LawfulMonad m]
     [Least? α] [LE α] [DecidableLE α] [UpwardEnumerable α] [Rxc.IsAlwaysFinite α]
     [LawfulUpwardEnumerable α] [LawfulUpwardEnumerableLeast? α] [LawfulUpwardEnumerableLE α]
     {xs : Ric α} {init : β} {f : α → β → m (ForInStep β)}
@@ -1170,7 +1172,7 @@ open Std Std.PRange in
 
 @[spec]
 theorem Spec.forIn'_rio {α β : Type u} {m : Type u → Type v} {Pred : Type u} {EPred : Type u}
-    [Monad m] [Assertion Pred] [Assertion EPred] [WPMonad m Pred EPred] [LawfulMonad m]
+    [Monad m] [Assertion Pred] [Assertion EPred] [∀ α, WP (m α) α Pred EPred] [WPMonad m Pred EPred] [LawfulMonad m]
     [Least? α] [LT α] [DecidableLT α] [UpwardEnumerable α] [Rxo.IsAlwaysFinite α]
     [LawfulUpwardEnumerable α] [LawfulUpwardEnumerableLeast? α] [LawfulUpwardEnumerableLT α]
     {xs : Rio α} {init : β} {f : (a : α) → a ∈ xs → β → m (ForInStep β)}
@@ -1196,7 +1198,7 @@ open Std Std.PRange in
 
 @[spec]
 theorem Spec.forIn_rio {α β : Type u} {m : Type u → Type v} {Pred : Type u} {EPred : Type u}
-    [Monad m] [Assertion Pred] [Assertion EPred] [WPMonad m Pred EPred] [LawfulMonad m]
+    [Monad m] [Assertion Pred] [Assertion EPred] [∀ α, WP (m α) α Pred EPred] [WPMonad m Pred EPred] [LawfulMonad m]
     [Least? α] [LT α] [DecidableLT α] [UpwardEnumerable α] [Rxo.IsAlwaysFinite α]
     [LawfulUpwardEnumerable α] [LawfulUpwardEnumerableLeast? α] [LawfulUpwardEnumerableLT α]
     {xs : Rio α} {init : β} {f : α → β → m (ForInStep β)}
@@ -1222,7 +1224,7 @@ open Std Std.PRange in
 
 @[spec]
 theorem Spec.forIn'_rii {α β : Type u} {m : Type u → Type v} {Pred : Type u} {EPred : Type u}
-    [Monad m] [Assertion Pred] [Assertion EPred] [WPMonad m Pred EPred] [LawfulMonad m]
+    [Monad m] [Assertion Pred] [Assertion EPred] [∀ α, WP (m α) α Pred EPred] [WPMonad m Pred EPred] [LawfulMonad m]
     [Least? α] [UpwardEnumerable α] [Rxi.IsAlwaysFinite α]
     [LawfulUpwardEnumerable α] [LawfulUpwardEnumerableLeast? α]
     {xs : Rii α} {init : β} {f : (a : α) → a ∈ xs → β → m (ForInStep β)}
@@ -1248,7 +1250,7 @@ open Std Std.PRange in
 
 @[spec]
 theorem Spec.forIn_rii {α β : Type u} {m : Type u → Type v} {Pred : Type u} {EPred : Type u}
-    [Monad m] [Assertion Pred] [Assertion EPred] [WPMonad m Pred EPred] [LawfulMonad m]
+    [Monad m] [Assertion Pred] [Assertion EPred] [∀ α, WP (m α) α Pred EPred] [WPMonad m Pred EPred] [LawfulMonad m]
     [Least? α] [UpwardEnumerable α] [Rxi.IsAlwaysFinite α]
     [LawfulUpwardEnumerable α] [LawfulUpwardEnumerableLeast? α]
     {xs : Rii α} {init : β} {f : α → β → m (ForInStep β)}
@@ -1274,7 +1276,7 @@ open Std Std.Iterators in
 
 @[spec]
 theorem Spec.forIn_slice {δ : Type u} {m : Type u → Type w} {Pred : Type u} {EPred : Type u}
-    [Monad m] [Assertion Pred] [Assertion EPred] [WPMonad m Pred EPred] [LawfulMonad m]
+    [Monad m] [Assertion Pred] [Assertion EPred] [∀ α, WP (m α) α Pred EPred] [WPMonad m Pred EPred] [LawfulMonad m]
     {γ : Type u'} {α β : Type u}
     [ToIterator (Slice γ) Id α β]
     [Iterator α Id β]
@@ -1304,7 +1306,7 @@ open Std Std.Iterators
 
 @[spec low]
 theorem Spec.forIn_iter {α β γ : Type u} {m : Type u → Type w} {Pred : Type u} {EPred : Type u}
-    [Monad m] [Assertion Pred] [Assertion EPred] [WPMonad m Pred EPred] [LawfulMonad m]
+    [Monad m] [Assertion Pred] [Assertion EPred] [∀ α, WP (m α) α Pred EPred] [WPMonad m Pred EPred] [LawfulMonad m]
     [Iterator α Id β] [Finite α Id] [IteratorLoop α Id m] [LawfulIteratorLoop α Id m]
     {init : γ} {f : β → γ → m (ForInStep γ)}
     {it : Iter (α := α) β}
@@ -1326,7 +1328,7 @@ theorem Spec.forIn_iter {α β γ : Type u} {m : Type u → Type w} {Pred : Type
 
 @[spec low]
 theorem Spec.forIn_iterM_id {α β γ : Type u} {m : Type u → Type w} {Pred : Type u} {EPred : Type u}
-    [Monad m] [Assertion Pred] [Assertion EPred] [WPMonad m Pred EPred] [LawfulMonad m]
+    [Monad m] [Assertion Pred] [Assertion EPred] [∀ α, WP (m α) α Pred EPred] [WPMonad m Pred EPred] [LawfulMonad m]
     [Iterator α Id β] [Finite α Id] [IteratorLoop α Id m] [LawfulIteratorLoop α Id m]
     {init : γ} {f : β → γ → m (ForInStep γ)}
     {it : IterM (α := α) Id β}
@@ -1350,7 +1352,7 @@ theorem Spec.forIn_iterM_id {α β γ : Type u} {m : Type u → Type w} {Pred : 
 
 @[spec low]
 theorem Spec.foldM_iter {α β γ : Type u} {m : Type u → Type w} {Pred : Type u} {EPred : Type u}
-    [Monad m] [Assertion Pred] [Assertion EPred] [WPMonad m Pred EPred] [LawfulMonad m]
+    [Monad m] [Assertion Pred] [Assertion EPred] [∀ α, WP (m α) α Pred EPred] [WPMonad m Pred EPred] [LawfulMonad m]
     [Iterator α Id β] [Finite α Id] [IteratorLoop α Id m] [LawfulIteratorLoop α Id m]
     {it : Iter (α := α) β}
     {init : γ} {f : γ → β → m γ}
@@ -1370,7 +1372,7 @@ theorem Spec.foldM_iter {α β γ : Type u} {m : Type u → Type w} {Pred : Type
 
 @[spec low]
 theorem Spec.foldM_iterM_id {α β γ : Type u} {m : Type u → Type w} {Pred : Type u} {EPred : Type u}
-    [Monad m] [Assertion Pred] [Assertion EPred] [WPMonad m Pred EPred] [LawfulMonad m]
+    [Monad m] [Assertion Pred] [Assertion EPred] [∀ α, WP (m α) α Pred EPred] [WPMonad m Pred EPred] [LawfulMonad m]
     [Iterator α Id β] [Finite α Id] [IteratorLoop α Id m] [LawfulIteratorLoop α Id m]
     {it : IterM (α := α) Id β}
     {init : γ} {f : γ → β → m γ}
@@ -1392,7 +1394,7 @@ theorem Spec.foldM_iterM_id {α β γ : Type u} {m : Type u → Type w} {Pred : 
 theorem Spec.IterM.forIn_filterMapWithPostcondition {α β β₂ γ : Type w}
     {m : Type w → Type w'} {n : Type w → Type w''} {o : Type w → Type w'''}
     {Pred : Type w} {EPred : Type w}
-    [Monad m] [LawfulMonad m] [Monad n] [LawfulMonad n] [Monad o] [LawfulMonad o] [Assertion Pred] [Assertion EPred] [WPMonad o Pred EPred]
+    [Monad m] [LawfulMonad m] [Monad n] [LawfulMonad n] [Monad o] [LawfulMonad o] [Assertion Pred] [Assertion EPred] [∀ α, WP (o α) α Pred EPred] [WPMonad o Pred EPred]
     [MonadLiftT m n] [LawfulMonadLiftT m n] [MonadLiftT n o] [LawfulMonadLiftT n o]
     [Iterator α m β] [Finite α m]
     [IteratorLoop α m o] [LawfulIteratorLoop α m o]
@@ -1412,7 +1414,7 @@ theorem Spec.IterM.forIn_filterMapWithPostcondition {α β β₂ γ : Type w}
 theorem Spec.IterM.forIn_filterMapM {α β β₂ γ : Type w}
     {m : Type w → Type w'} {n : Type w → Type w''} {o : Type w → Type w'''}
     {Pred : Type w} {EPred : Type w}
-    [Monad m] [LawfulMonad m] [Monad n] [LawfulMonad n] [Monad o] [LawfulMonad o] [Assertion Pred] [Assertion EPred] [WPMonad o Pred EPred]
+    [Monad m] [LawfulMonad m] [Monad n] [LawfulMonad n] [Monad o] [LawfulMonad o] [Assertion Pred] [Assertion EPred] [∀ α, WP (o α) α Pred EPred] [WPMonad o Pred EPred]
     [MonadAttach n] [WeaklyLawfulMonadAttach n]
     [MonadLiftT m n] [LawfulMonadLiftT m n] [MonadLiftT n o] [LawfulMonadLiftT n o]
     [Iterator α m β] [Finite α m]
@@ -1433,7 +1435,7 @@ theorem Spec.IterM.forIn_filterMapM {α β β₂ γ : Type w}
 theorem Spec.IterM.forIn_filterMap {α β β₂ γ : Type w}
     {m : Type w → Type w'} {n : Type w → Type w''}
     {Pred : Type w} {EPred : Type w}
-    [Monad m] [LawfulMonad m] [Monad n] [LawfulMonad n] [Assertion Pred] [Assertion EPred] [WPMonad n Pred EPred]
+    [Monad m] [LawfulMonad m] [Monad n] [LawfulMonad n] [Assertion Pred] [Assertion EPred] [∀ α, WP (n α) α Pred EPred] [WPMonad n Pred EPred]
     [MonadLiftT m n] [LawfulMonadLiftT m n]
     [Iterator α m β] [Finite α m]
     [IteratorLoop α m n] [LawfulIteratorLoop α m n]
@@ -1451,7 +1453,7 @@ theorem Spec.IterM.forIn_filterMap {α β β₂ γ : Type w}
 theorem Spec.IterM.forIn_mapWithPostcondition {α β β₂ γ : Type w}
     {m : Type w → Type w'} {n : Type w → Type w''} {o : Type w → Type w'''}
     {Pred : Type w} {EPred : Type w}
-    [Monad m] [LawfulMonad m] [Monad n] [LawfulMonad n] [Monad o] [LawfulMonad o] [Assertion Pred] [Assertion EPred] [WPMonad o Pred EPred]
+    [Monad m] [LawfulMonad m] [Monad n] [LawfulMonad n] [Monad o] [LawfulMonad o] [Assertion Pred] [Assertion EPred] [∀ α, WP (o α) α Pred EPred] [WPMonad o Pred EPred]
     [MonadLiftT m n] [LawfulMonadLiftT m n] [MonadLiftT n o] [LawfulMonadLiftT n o]
     [Iterator α m β] [Finite α m]
     [IteratorLoop α m o] [LawfulIteratorLoop α m o]
@@ -1468,7 +1470,7 @@ theorem Spec.IterM.forIn_mapWithPostcondition {α β β₂ γ : Type w}
 theorem Spec.IterM.forIn_mapM {α β β₂ γ : Type w}
     {m : Type w → Type w'} {n : Type w → Type w''} {o : Type w → Type w'''}
     {Pred : Type w} {EPred : Type w}
-    [Monad m] [LawfulMonad m] [Monad n] [LawfulMonad n] [Monad o] [LawfulMonad o] [Assertion Pred] [Assertion EPred] [WPMonad o Pred EPred]
+    [Monad m] [LawfulMonad m] [Monad n] [LawfulMonad n] [Monad o] [LawfulMonad o] [Assertion Pred] [Assertion EPred] [∀ α, WP (o α) α Pred EPred] [WPMonad o Pred EPred]
     [MonadAttach n] [WeaklyLawfulMonadAttach n]
     [MonadLiftT m n] [LawfulMonadLiftT m n] [MonadLiftT n o] [LawfulMonadLiftT n o]
     [Iterator α m β] [Finite α m]
@@ -1486,7 +1488,7 @@ theorem Spec.IterM.forIn_mapM {α β β₂ γ : Type w}
 theorem Spec.IterM.forIn_map {α β β₂ γ : Type w}
     {m : Type w → Type w'} {n : Type w → Type w''}
     {Pred : Type w} {EPred : Type w}
-    [Monad m] [LawfulMonad m] [Monad n] [LawfulMonad n] [Assertion Pred] [Assertion EPred] [WPMonad n Pred EPred]
+    [Monad m] [LawfulMonad m] [Monad n] [LawfulMonad n] [Assertion Pred] [Assertion EPred] [∀ α, WP (n α) α Pred EPred] [WPMonad n Pred EPred]
     [MonadLiftT m n] [LawfulMonadLiftT m n]
     [Iterator α m β] [Finite α m] [IteratorLoop α m n] [LawfulIteratorLoop α m n]
     {it : IterM (α := α) m β} {f : β → β₂} {init : γ} {g : β₂ → γ → n (ForInStep γ)}
@@ -1500,7 +1502,7 @@ theorem Spec.IterM.forIn_map {α β β₂ γ : Type w}
 theorem Spec.IterM.forIn_filterWithPostcondition {α β γ : Type w}
     {m : Type w → Type w'} {n : Type w → Type w''} {o : Type w → Type w'''}
     {Pred : Type w} {EPred : Type w}
-    [Monad m] [LawfulMonad m] [Monad n] [LawfulMonad n] [Monad o] [LawfulMonad o] [Assertion Pred] [Assertion EPred] [WPMonad o Pred EPred]
+    [Monad m] [LawfulMonad m] [Monad n] [LawfulMonad n] [Monad o] [LawfulMonad o] [Assertion Pred] [Assertion EPred] [∀ α, WP (o α) α Pred EPred] [WPMonad o Pred EPred]
     [MonadLiftT m n] [LawfulMonadLiftT m n] [MonadLiftT n o] [LawfulMonadLiftT n o]
     [Iterator α m β] [Finite α m]
     [IteratorLoop α m o] [LawfulIteratorLoop α m o]
@@ -1517,7 +1519,7 @@ theorem Spec.IterM.forIn_filterWithPostcondition {α β γ : Type w}
 theorem Spec.IterM.forIn_filterM {α β γ : Type w}
     {m : Type w → Type w'} {n : Type w → Type w''} {o : Type w → Type w'''}
     {Pred : Type w} {EPred : Type w}
-    [Monad m] [LawfulMonad m] [Monad n] [LawfulMonad n] [Monad o] [LawfulMonad o] [Assertion Pred] [Assertion EPred] [WPMonad o Pred EPred]
+    [Monad m] [LawfulMonad m] [Monad n] [LawfulMonad n] [Monad o] [LawfulMonad o] [Assertion Pred] [Assertion EPred] [∀ α, WP (o α) α Pred EPred] [WPMonad o Pred EPred]
     [MonadAttach n] [WeaklyLawfulMonadAttach n]
     [MonadLiftT m n] [LawfulMonadLiftT m n] [MonadLiftT n o] [LawfulMonadLiftT n o]
     [Iterator α m β] [Finite α m]
@@ -1535,7 +1537,7 @@ theorem Spec.IterM.forIn_filterM {α β γ : Type w}
 theorem Spec.IterM.forIn_filter {α β γ : Type w}
     {m : Type w → Type w'} {n : Type w → Type w''}
     {Pred : Type w} {EPred : Type w}
-    [Monad m] [LawfulMonad m] [Monad n] [LawfulMonad n] [Assertion Pred] [Assertion EPred] [WPMonad n Pred EPred]
+    [Monad m] [LawfulMonad m] [Monad n] [LawfulMonad n] [Assertion Pred] [Assertion EPred] [∀ α, WP (n α) α Pred EPred] [WPMonad n Pred EPred]
     [MonadLiftT m n] [LawfulMonadLiftT m n]
     [Iterator α m β] [Finite α m] [IteratorLoop α m n] [LawfulIteratorLoop α m n]
     {it : IterM (α := α) m β} {f : β → Bool} {init : γ} {g : β → γ → n (ForInStep γ)}
@@ -1550,7 +1552,7 @@ theorem Spec.IterM.foldM_filterMapWithPostcondition {α β γ δ : Type w}
     {m : Type w → Type w'} {n : Type w → Type w''} {o : Type w → Type w'''}
     {Pred : Type w} {EPred : Type w}
     [Iterator α m β] [Finite α m]
-    [Monad m] [Monad n] [Monad o] [LawfulMonad m] [LawfulMonad n] [LawfulMonad o] [Assertion Pred] [Assertion EPred] [WPMonad o Pred EPred]
+    [Monad m] [Monad n] [Monad o] [LawfulMonad m] [LawfulMonad n] [LawfulMonad o] [Assertion Pred] [Assertion EPred] [∀ α, WP (o α) α Pred EPred] [WPMonad o Pred EPred]
     [IteratorLoop α m n] [IteratorLoop α m o]
     [LawfulIteratorLoop α m n] [LawfulIteratorLoop α m o]
     [MonadLiftT m n] [MonadLiftT n o] [LawfulMonadLiftT m n] [LawfulMonadLiftT n o]
@@ -1572,7 +1574,7 @@ theorem Spec.IterM.foldM_filterMapM {α β γ δ : Type w}
     [Iterator α m β] [Finite α m]
     [Monad m] [LawfulMonad m]
     [Monad n] [MonadAttach n] [LawfulMonad n] [WeaklyLawfulMonadAttach n]
-    [Monad o] [LawfulMonad o] [Assertion Pred] [Assertion EPred] [WPMonad o Pred EPred]
+    [Monad o] [LawfulMonad o] [Assertion Pred] [Assertion EPred] [∀ α, WP (o α) α Pred EPred] [WPMonad o Pred EPred]
     [IteratorLoop α m n] [IteratorLoop α m o]
     [LawfulIteratorLoop α m n] [LawfulIteratorLoop α m o]
     [MonadLiftT m n] [MonadLiftT n o] [LawfulMonadLiftT m n] [LawfulMonadLiftT n o]
@@ -1592,7 +1594,7 @@ theorem Spec.IterM.foldM_mapWithPostcondition {α β γ δ : Type w}
     {m : Type w → Type w'} {n : Type w → Type w''} {o : Type w → Type w'''}
     {Pred : Type w} {EPred : Type w}
     [Iterator α m β] [Finite α m]
-    [Monad m] [Monad n] [Monad o] [LawfulMonad m] [LawfulMonad n] [LawfulMonad o] [Assertion Pred] [Assertion EPred] [WPMonad o Pred EPred]
+    [Monad m] [Monad n] [Monad o] [LawfulMonad m] [LawfulMonad n] [LawfulMonad o] [Assertion Pred] [Assertion EPred] [∀ α, WP (o α) α Pred EPred] [WPMonad o Pred EPred]
     [IteratorLoop α m n] [IteratorLoop α m o]
     [LawfulIteratorLoop α m n] [LawfulIteratorLoop α m o]
     [MonadLiftT m n] [MonadLiftT n o] [LawfulMonadLiftT m n] [LawfulMonadLiftT n o]
@@ -1612,7 +1614,7 @@ theorem Spec.IterM.foldM_mapM {α β γ δ : Type w}
     [Iterator α m β] [Finite α m]
     [Monad m] [LawfulMonad m]
     [Monad n] [MonadAttach n] [LawfulMonad n] [WeaklyLawfulMonadAttach n]
-    [Monad o] [LawfulMonad o] [Assertion Pred] [Assertion EPred] [WPMonad o Pred EPred]
+    [Monad o] [LawfulMonad o] [Assertion Pred] [Assertion EPred] [∀ α, WP (o α) α Pred EPred] [WPMonad o Pred EPred]
     [IteratorLoop α m n] [IteratorLoop α m o]
     [LawfulIteratorLoop α m n] [LawfulIteratorLoop α m o]
     [MonadLiftT m n] [MonadLiftT n o] [LawfulMonadLiftT m n] [LawfulMonadLiftT n o]
@@ -1630,7 +1632,7 @@ theorem Spec.IterM.foldM_filterWithPostcondition {α β δ : Type w}
     {m : Type w → Type w'} {n : Type w → Type w''} {o : Type w → Type w'''}
     {Pred : Type w} {EPred : Type w}
     [Iterator α m β] [Finite α m]
-    [Monad m] [Monad n] [Monad o] [LawfulMonad m] [LawfulMonad n] [LawfulMonad o] [Assertion Pred] [Assertion EPred] [WPMonad o Pred EPred]
+    [Monad m] [Monad n] [Monad o] [LawfulMonad m] [LawfulMonad n] [LawfulMonad o] [Assertion Pred] [Assertion EPred] [∀ α, WP (o α) α Pred EPred] [WPMonad o Pred EPred]
     [IteratorLoop α m n] [IteratorLoop α m o]
     [LawfulIteratorLoop α m n] [LawfulIteratorLoop α m o]
     [MonadLiftT m n] [MonadLiftT n o] [LawfulMonadLiftT m n] [LawfulMonadLiftT n o]
@@ -1650,7 +1652,7 @@ theorem Spec.IterM.foldM_filterM {α β δ : Type w}
     [Iterator α m β] [Finite α m]
     [Monad m] [LawfulMonad m]
     [Monad n] [MonadAttach n] [LawfulMonad n] [WeaklyLawfulMonadAttach n]
-    [Monad o] [LawfulMonad o] [Assertion Pred] [Assertion EPred] [WPMonad o Pred EPred]
+    [Monad o] [LawfulMonad o] [Assertion Pred] [Assertion EPred] [∀ α, WP (o α) α Pred EPred] [WPMonad o Pred EPred]
     [IteratorLoop α m n] [IteratorLoop α m o]
     [LawfulIteratorLoop α m n] [LawfulIteratorLoop α m o]
     [MonadLiftT m n] [MonadLiftT n o] [LawfulMonadLiftT m n] [LawfulMonadLiftT n o]
@@ -1667,7 +1669,7 @@ theorem Spec.IterM.foldM_filterM {α β δ : Type w}
 theorem Spec.IterM.foldM_filterMap {α β γ δ : Type w}
     {m : Type w → Type w'} {n : Type w → Type w''}
     {Pred : Type w} {EPred : Type w}
-    [Iterator α m β] [Finite α m] [Monad m] [Monad n] [LawfulMonad m] [LawfulMonad n] [Assertion Pred] [Assertion EPred] [WPMonad n Pred EPred]
+    [Iterator α m β] [Finite α m] [Monad m] [Monad n] [LawfulMonad m] [LawfulMonad n] [Assertion Pred] [Assertion EPred] [∀ α, WP (n α) α Pred EPred] [WPMonad n Pred EPred]
     [IteratorLoop α m n]
     [LawfulIteratorLoop α m n]
     [MonadLiftT m n] [LawfulMonadLiftT m n]
@@ -1684,7 +1686,7 @@ theorem Spec.IterM.foldM_filterMap {α β γ δ : Type w}
 theorem Spec.IterM.foldM_map {α β γ δ : Type w}
     {m : Type w → Type w'} {n : Type w → Type w''}
     {Pred : Type w} {EPred : Type w}
-    [Iterator α m β] [Finite α m] [Monad m] [Monad n] [LawfulMonad m] [LawfulMonad n] [Assertion Pred] [Assertion EPred] [WPMonad n Pred EPred]
+    [Iterator α m β] [Finite α m] [Monad m] [Monad n] [LawfulMonad m] [LawfulMonad n] [Assertion Pred] [Assertion EPred] [∀ α, WP (n α) α Pred EPred] [WPMonad n Pred EPred]
     [IteratorLoop α m n] [LawfulIteratorLoop α m n]
     [MonadLiftT m n] [LawfulMonadLiftT m n]
     {f : β → γ} {g : δ → γ → n δ} {init : δ} {it : IterM (α := α) m β}
@@ -1698,7 +1700,7 @@ theorem Spec.IterM.foldM_map {α β γ δ : Type w}
 theorem Spec.IterM.foldM_filter {α β δ : Type w}
     {m : Type w → Type w'} {n : Type w → Type w''}
     {Pred : Type w} {EPred : Type w}
-    [Iterator α m β] [Finite α m] [Monad m] [Monad n] [LawfulMonad m] [LawfulMonad n] [Assertion Pred] [Assertion EPred] [WPMonad n Pred EPred]
+    [Iterator α m β] [Finite α m] [Monad m] [Monad n] [LawfulMonad m] [LawfulMonad n] [Assertion Pred] [Assertion EPred] [∀ α, WP (n α) α Pred EPred] [WPMonad n Pred EPred]
     [IteratorLoop α m n]
     [LawfulIteratorLoop α m n]
     [MonadLiftT m n] [LawfulMonadLiftT m n]
@@ -1715,7 +1717,7 @@ theorem Spec.IterM.fold_filterMapWithPostcondition {α β γ δ : Type w}
     {Pred : Type w} {EPred : Type w}
     [Iterator α m β] [Finite α m]
     [Monad m] [LawfulMonad m]
-    [Monad n] [LawfulMonad n] [Assertion Pred] [Assertion EPred] [WPMonad n Pred EPred]
+    [Monad n] [LawfulMonad n] [Assertion Pred] [Assertion EPred] [∀ α, WP (n α) α Pred EPred] [WPMonad n Pred EPred]
     [IteratorLoop α m n] [LawfulIteratorLoop α m n]
     [MonadLiftT m n] [LawfulMonadLiftT m n]
     {f : β → PostconditionT n (Option γ)} {g : δ → γ → δ} {init : δ} {it : IterM (α := α) m β}
@@ -1733,7 +1735,7 @@ theorem Spec.IterM.fold_filterMapM {α β γ δ : Type w}
     {Pred : Type w} {EPred : Type w}
     [Iterator α m β] [Finite α m]
     [Monad m] [LawfulMonad m]
-    [Monad n] [MonadAttach n] [LawfulMonad n] [WeaklyLawfulMonadAttach n] [Assertion Pred] [Assertion EPred] [WPMonad n Pred EPred]
+    [Monad n] [MonadAttach n] [LawfulMonad n] [WeaklyLawfulMonadAttach n] [Assertion Pred] [Assertion EPred] [∀ α, WP (n α) α Pred EPred] [WPMonad n Pred EPred]
     [IteratorLoop α m n] [LawfulIteratorLoop α m n]
     [MonadLiftT m n] [LawfulMonadLiftT m n]
     {f : β → n (Option γ)} {g : δ → γ → δ} {init : δ} {it : IterM (α := α) m β}
@@ -1751,7 +1753,7 @@ theorem Spec.IterM.fold_mapWithPostcondition {α β γ δ : Type w}
     {Pred : Type w} {EPred : Type w}
     [Iterator α m β] [Finite α m]
     [Monad m] [LawfulMonad m]
-    [Monad n] [LawfulMonad n] [Assertion Pred] [Assertion EPred] [WPMonad n Pred EPred]
+    [Monad n] [LawfulMonad n] [Assertion Pred] [Assertion EPred] [∀ α, WP (n α) α Pred EPred] [WPMonad n Pred EPred]
     [IteratorLoop α m n] [LawfulIteratorLoop α m n]
     [MonadLiftT m n] [LawfulMonadLiftT m n]
     {f : β → PostconditionT n γ} {g : δ → γ → δ} {init : δ} {it : IterM (α := α) m β}
@@ -1767,7 +1769,7 @@ theorem Spec.IterM.fold_mapM {α β γ δ : Type w}
     {Pred : Type w} {EPred : Type w}
     [Iterator α m β] [Finite α m]
     [Monad m] [LawfulMonad m]
-    [Monad n] [MonadAttach n] [LawfulMonad n] [WeaklyLawfulMonadAttach n] [Assertion Pred] [Assertion EPred] [WPMonad n Pred EPred]
+    [Monad n] [MonadAttach n] [LawfulMonad n] [WeaklyLawfulMonadAttach n] [Assertion Pred] [Assertion EPred] [∀ α, WP (n α) α Pred EPred] [WPMonad n Pred EPred]
     [IteratorLoop α m n] [LawfulIteratorLoop α m n]
     [MonadLiftT m n] [LawfulMonadLiftT m n]
     {f : β → n γ} {g : δ → γ → δ} {init : δ} {it : IterM (α := α) m β}
@@ -1783,7 +1785,7 @@ theorem Spec.IterM.fold_filterWithPostcondition {α β δ : Type w}
     {Pred : Type w} {EPred : Type w}
     [Iterator α m β] [Finite α m]
     [Monad m] [LawfulMonad m]
-    [Monad n] [LawfulMonad n] [Assertion Pred] [Assertion EPred] [WPMonad n Pred EPred]
+    [Monad n] [LawfulMonad n] [Assertion Pred] [Assertion EPred] [∀ α, WP (n α) α Pred EPred] [WPMonad n Pred EPred]
     [IteratorLoop α m n] [LawfulIteratorLoop α m n]
     [MonadLiftT m n] [LawfulMonadLiftT m n]
     {f : β → PostconditionT n (ULift Bool)} {g : δ → β → δ} {init : δ} {it : IterM (α := α) m β}
@@ -1799,7 +1801,7 @@ theorem Spec.IterM.fold_filterM {α β δ : Type w}
     {Pred : Type w} {EPred : Type w}
     [Iterator α m β] [Finite α m]
     [Monad m] [LawfulMonad m]
-    [Monad n] [MonadAttach n] [LawfulMonad n] [WeaklyLawfulMonadAttach n] [Assertion Pred] [Assertion EPred] [WPMonad n Pred EPred]
+    [Monad n] [MonadAttach n] [LawfulMonad n] [WeaklyLawfulMonadAttach n] [Assertion Pred] [Assertion EPred] [∀ α, WP (n α) α Pred EPred] [WPMonad n Pred EPred]
     [IteratorLoop α m n] [LawfulIteratorLoop α m n]
     [MonadLiftT m n] [LawfulMonadLiftT m n]
     {f : β → n (ULift Bool)} {g : δ → β → δ} {init : δ} {it : IterM (α := α) m β}
@@ -1813,7 +1815,7 @@ theorem Spec.IterM.fold_filterM {α β δ : Type w}
 theorem Spec.IterM.fold_filterMap {α β γ δ : Type w}
     {m : Type w → Type w'}
     {Pred : Type w} {EPred : Type w}
-    [Iterator α m β] [Finite α m] [Monad m] [LawfulMonad m] [Assertion Pred] [Assertion EPred] [WPMonad m Pred EPred]
+    [Iterator α m β] [Finite α m] [Monad m] [LawfulMonad m] [Assertion Pred] [Assertion EPred] [∀ α, WP (m α) α Pred EPred] [WPMonad m Pred EPred]
     [IteratorLoop α m m] [LawfulIteratorLoop α m m]
     {f : β → Option γ} {g : δ → γ → δ} {init : δ} {it : IterM (α := α) m β}
     {P : Pred} {Q : δ → Pred} {eQ : EPred}
@@ -1829,7 +1831,7 @@ theorem Spec.IterM.fold_filterMap {α β γ δ : Type w}
 theorem Spec.IterM.fold_map {α β γ δ : Type w}
     {m : Type w → Type w'}
     {Pred : Type w} {EPred : Type w}
-    [Iterator α m β] [Finite α m] [Monad m] [LawfulMonad m] [Assertion Pred] [Assertion EPred] [WPMonad m Pred EPred]
+    [Iterator α m β] [Finite α m] [Monad m] [LawfulMonad m] [Assertion Pred] [Assertion EPred] [∀ α, WP (m α) α Pred EPred] [WPMonad m Pred EPred]
     [IteratorLoop α m m] [LawfulIteratorLoop α m m]
     {f : β → γ} {g : δ → γ → δ} {init : δ} {it : IterM (α := α) m β}
     {P : Pred} {Q : δ → Pred} {eQ : EPred}
@@ -1842,7 +1844,7 @@ theorem Spec.IterM.fold_map {α β γ δ : Type w}
 theorem Spec.IterM.fold_filter {α β δ : Type w}
     {m : Type w → Type w'}
     {Pred : Type w} {EPred : Type w}
-    [Iterator α m β] [Finite α m] [Monad m] [LawfulMonad m] [Assertion Pred] [Assertion EPred] [WPMonad m Pred EPred]
+    [Iterator α m β] [Finite α m] [Monad m] [LawfulMonad m] [Assertion Pred] [Assertion EPred] [∀ α, WP (m α) α Pred EPred] [WPMonad m Pred EPred]
     [IteratorLoop α m m] [LawfulIteratorLoop α m m]
     {f : β → Bool} {g : δ → β → δ} {init : δ} {it : IterM (α := α) m β}
     {P : Pred} {Q : δ → Pred} {eQ : EPred}
@@ -1856,7 +1858,7 @@ theorem Spec.Iter.forIn_filterMapWithPostcondition {α β β₂ γ : Type w}
     {n : Type w → Type w'} {o : Type w → Type w''}
     {Pred : Type w} {EPred : Type w}
     [Iterator α Id β]
-    [Monad n] [LawfulMonad n] [Monad o] [LawfulMonad o] [Assertion Pred] [Assertion EPred] [WPMonad o Pred EPred]
+    [Monad n] [LawfulMonad n] [Monad o] [LawfulMonad o] [Assertion Pred] [Assertion EPred] [∀ α, WP (o α) α Pred EPred] [WPMonad o Pred EPred]
     [MonadLiftT n o] [LawfulMonadLiftT n o] [Finite α Id]
     [IteratorLoop α Id o] [LawfulIteratorLoop α Id o]
     {it : Iter (α := α) β} {f : β → PostconditionT n (Option β₂)} {init : γ}
@@ -1874,7 +1876,7 @@ theorem Spec.Iter.forIn_filterMapM {α β β₂ γ : Type w}
     {n : Type w → Type w'} {o : Type w → Type w''}
     {Pred : Type w} {EPred : Type w}
     [Iterator α Id β]
-    [Monad n] [LawfulMonad n] [Monad o] [LawfulMonad o] [Assertion Pred] [Assertion EPred] [WPMonad o Pred EPred]
+    [Monad n] [LawfulMonad n] [Monad o] [LawfulMonad o] [Assertion Pred] [Assertion EPred] [∀ α, WP (o α) α Pred EPred] [WPMonad o Pred EPred]
     [MonadAttach n] [WeaklyLawfulMonadAttach n]
     [MonadLiftT n o] [LawfulMonadLiftT n o]
     [Finite α Id] [IteratorLoop α Id o] [LawfulIteratorLoop α Id o]
@@ -1893,7 +1895,7 @@ theorem Spec.Iter.forIn_filterMap {α β β₂ γ : Type w}
     {n : Type w → Type w'}
     {Pred : Type w} {EPred : Type w}
     [Iterator α Id β]
-    [Monad n] [LawfulMonad n] [Assertion Pred] [Assertion EPred] [WPMonad n Pred EPred] [Finite α Id]
+    [Monad n] [LawfulMonad n] [Assertion Pred] [Assertion EPred] [∀ α, WP (n α) α Pred EPred] [WPMonad n Pred EPred] [Finite α Id]
     [IteratorLoop α Id n] [LawfulIteratorLoop α Id n]
     {it : Iter (α := α) β} {f : β → Option β₂} {init : γ} {g : β₂ → γ → n (ForInStep γ)}
     {P : Pred} {Q : γ → Pred} {eQ : EPred}
@@ -1910,7 +1912,7 @@ theorem Spec.Iter.forIn_mapWithPostcondition {α β β₂ γ : Type w}
     {n : Type w → Type w'} {o : Type w → Type w''}
     {Pred : Type w} {EPred : Type w}
     [Iterator α Id β]
-    [Monad n] [LawfulMonad n] [Monad o] [LawfulMonad o] [Assertion Pred] [Assertion EPred] [WPMonad o Pred EPred]
+    [Monad n] [LawfulMonad n] [Monad o] [LawfulMonad o] [Assertion Pred] [Assertion EPred] [∀ α, WP (o α) α Pred EPred] [WPMonad o Pred EPred]
     [MonadLiftT n o] [LawfulMonadLiftT n o] [Finite α Id]
     [IteratorLoop α Id o] [LawfulIteratorLoop α Id o]
     {it : Iter (α := α) β} {f : β → PostconditionT n β₂} {init : γ}
@@ -1925,7 +1927,7 @@ theorem Spec.Iter.forIn_mapM {α β β₂ γ : Type w}
     {n : Type w → Type w'} {o : Type w → Type w''}
     {Pred : Type w} {EPred : Type w}
     [Iterator α Id β]
-    [Monad n] [LawfulMonad n] [Monad o] [LawfulMonad o] [Assertion Pred] [Assertion EPred] [WPMonad o Pred EPred]
+    [Monad n] [LawfulMonad n] [Monad o] [LawfulMonad o] [Assertion Pred] [Assertion EPred] [∀ α, WP (o α) α Pred EPred] [WPMonad o Pred EPred]
     [MonadAttach n] [WeaklyLawfulMonadAttach n]
     [MonadLiftT n o] [LawfulMonadLiftT n o]
     [Finite α Id]
@@ -1942,7 +1944,7 @@ theorem Spec.Iter.forIn_map {α β β₂ γ : Type w}
     {n : Type w → Type w'}
     {Pred : Type w} {EPred : Type w}
     [Iterator α Id β]
-    [Monad n] [LawfulMonad n] [Assertion Pred] [Assertion EPred] [WPMonad n Pred EPred]
+    [Monad n] [LawfulMonad n] [Assertion Pred] [Assertion EPred] [∀ α, WP (n α) α Pred EPred] [WPMonad n Pred EPred]
     [Finite α Id] [IteratorLoop α Id n] [LawfulIteratorLoop α Id n]
     {it : Iter (α := α) β} {f : β → β₂} {init : γ} {g : β₂ → γ → n (ForInStep γ)}
     {P : Pred} {Q : γ → Pred} {eQ : EPred}
@@ -1956,7 +1958,7 @@ theorem Spec.Iter.forIn_filterWithPostcondition {α β γ : Type w}
     {n : Type w → Type w'} {o : Type w → Type w''}
     {Pred : Type w} {EPred : Type w}
     [Iterator α Id β]
-    [Monad n] [LawfulMonad n] [Monad o] [LawfulMonad o] [Assertion Pred] [Assertion EPred] [WPMonad o Pred EPred]
+    [Monad n] [LawfulMonad n] [Monad o] [LawfulMonad o] [Assertion Pred] [Assertion EPred] [∀ α, WP (o α) α Pred EPred] [WPMonad o Pred EPred]
     [MonadLiftT n o] [LawfulMonadLiftT n o]
     [Finite α Id] [IteratorLoop α Id o] [LawfulIteratorLoop α Id o]
     {it : Iter (α := α) β} {f : β → PostconditionT n (ULift Bool)} {init : γ}
@@ -1971,7 +1973,7 @@ theorem Spec.Iter.forIn_filterM {α β γ : Type w}
     {n : Type w → Type w'} {o : Type w → Type w''}
     {Pred : Type w} {EPred : Type w}
     [Iterator α Id β]
-    [Monad n] [LawfulMonad n] [Monad o] [LawfulMonad o] [Assertion Pred] [Assertion EPred] [WPMonad o Pred EPred]
+    [Monad n] [LawfulMonad n] [Monad o] [LawfulMonad o] [Assertion Pred] [Assertion EPred] [∀ α, WP (o α) α Pred EPred] [WPMonad o Pred EPred]
     [MonadAttach n] [WeaklyLawfulMonadAttach n]
     [MonadLiftT n o] [LawfulMonadLiftT n o] [Finite α Id]
     [IteratorLoop α Id o] [LawfulIteratorLoop α Id o]
@@ -1987,7 +1989,7 @@ theorem Spec.Iter.forIn_filter {α β γ : Type w}
     {n : Type w → Type w'}
     {Pred : Type w} {EPred : Type w}
     [Iterator α Id β]
-    [Monad n] [LawfulMonad n] [Assertion Pred] [Assertion EPred] [WPMonad n Pred EPred]
+    [Monad n] [LawfulMonad n] [Assertion Pred] [Assertion EPred] [∀ α, WP (n α) α Pred EPred] [WPMonad n Pred EPred]
     [Finite α Id] [IteratorLoop α Id n] [LawfulIteratorLoop α Id n]
     {it : Iter (α := α) β} {f : β → Bool} {init : γ} {g : β → γ → n (ForInStep γ)}
     {P : Pred} {Q : γ → Pred} {eQ : EPred}
@@ -2001,7 +2003,7 @@ theorem Spec.Iter.foldM_filterMapWithPostcondition {α β γ δ : Type w}
     {n : Type w → Type w'} {o : Type w → Type w''}
     {Pred : Type w} {EPred : Type w}
     [Iterator α Id β] [Finite α Id]
-    [Monad n] [Monad o] [LawfulMonad n] [LawfulMonad o] [Assertion Pred] [Assertion EPred] [WPMonad o Pred EPred]
+    [Monad n] [Monad o] [LawfulMonad n] [LawfulMonad o] [Assertion Pred] [Assertion EPred] [∀ α, WP (o α) α Pred EPred] [WPMonad o Pred EPred]
     [IteratorLoop α Id n] [IteratorLoop α Id o]
     [LawfulIteratorLoop α Id n] [LawfulIteratorLoop α Id o]
     [MonadLiftT n o] [LawfulMonadLiftT n o]
@@ -2020,7 +2022,7 @@ theorem Spec.Iter.foldM_filterMapM {α β γ δ : Type w}
     {Pred : Type w} {EPred : Type w}
     [Iterator α Id β] [Finite α Id]
     [Monad n] [MonadAttach n] [LawfulMonad n] [WeaklyLawfulMonadAttach n]
-    [Monad o] [LawfulMonad o] [Assertion Pred] [Assertion EPred] [WPMonad o Pred EPred]
+    [Monad o] [LawfulMonad o] [Assertion Pred] [Assertion EPred] [∀ α, WP (o α) α Pred EPred] [WPMonad o Pred EPred]
     [IteratorLoop α Id n] [IteratorLoop α Id o]
     [LawfulIteratorLoop α Id n] [LawfulIteratorLoop α Id o]
     [MonadLiftT n o] [LawfulMonadLiftT n o]
@@ -2038,7 +2040,7 @@ theorem Spec.Iter.foldM_mapWithPostcondition {α β γ δ : Type w}
     {m : Type w → Type w'''} {n : Type w → Type w'} {o : Type w → Type w''}
     {Pred : Type w} {EPred : Type w}
     [Iterator α Id β] [Finite α Id]
-    [Monad m] [Monad n] [Monad o] [LawfulMonad m] [LawfulMonad n] [LawfulMonad o] [Assertion Pred] [Assertion EPred] [WPMonad o Pred EPred]
+    [Monad m] [Monad n] [Monad o] [LawfulMonad m] [LawfulMonad n] [LawfulMonad o] [Assertion Pred] [Assertion EPred] [∀ α, WP (o α) α Pred EPred] [WPMonad o Pred EPred]
     [IteratorLoop α Id n] [IteratorLoop α Id o]
     [LawfulIteratorLoop α Id n] [LawfulIteratorLoop α Id o]
     [MonadLiftT n o] [LawfulMonadLiftT n o]
@@ -2055,7 +2057,7 @@ theorem Spec.Iter.foldM_mapM {α β γ δ : Type w}
     {Pred : Type w} {EPred : Type w}
     [Iterator α Id β] [Finite α Id]
     [Monad n] [MonadAttach n] [LawfulMonad n] [WeaklyLawfulMonadAttach n]
-    [Monad o] [LawfulMonad o] [Assertion Pred] [Assertion EPred] [WPMonad o Pred EPred]
+    [Monad o] [LawfulMonad o] [Assertion Pred] [Assertion EPred] [∀ α, WP (o α) α Pred EPred] [WPMonad o Pred EPred]
     [IteratorLoop α Id n] [IteratorLoop α Id o]
     [LawfulIteratorLoop α Id n] [LawfulIteratorLoop α Id o]
     [MonadLiftT n o] [LawfulMonadLiftT n o]
@@ -2071,7 +2073,7 @@ theorem Spec.Iter.foldM_filterWithPostcondition {α β δ : Type w}
     {n : Type w → Type w'} {o : Type w → Type w''}
     {Pred : Type w} {EPred : Type w}
     [Iterator α Id β] [Finite α Id]
-    [Monad n] [Monad o] [LawfulMonad n] [LawfulMonad o] [Assertion Pred] [Assertion EPred] [WPMonad o Pred EPred]
+    [Monad n] [Monad o] [LawfulMonad n] [LawfulMonad o] [Assertion Pred] [Assertion EPred] [∀ α, WP (o α) α Pred EPred] [WPMonad o Pred EPred]
     [IteratorLoop α Id n] [IteratorLoop α Id o]
     [LawfulIteratorLoop α Id n] [LawfulIteratorLoop α Id o]
     [MonadLiftT n o] [LawfulMonadLiftT n o]
@@ -2088,7 +2090,7 @@ theorem Spec.Iter.foldM_filterM {α β δ : Type w}
     {Pred : Type w} {EPred : Type w}
     [Iterator α Id β] [Finite α Id]
     [Monad n] [MonadAttach n] [LawfulMonad n] [WeaklyLawfulMonadAttach n]
-    [Monad o] [LawfulMonad o] [Assertion Pred] [Assertion EPred] [WPMonad o Pred EPred]
+    [Monad o] [LawfulMonad o] [Assertion Pred] [Assertion EPred] [∀ α, WP (o α) α Pred EPred] [WPMonad o Pred EPred]
     [IteratorLoop α Id n] [IteratorLoop α Id o]
     [LawfulIteratorLoop α Id n] [LawfulIteratorLoop α Id o]
     [MonadLiftT n o] [LawfulMonadLiftT n o]
@@ -2103,7 +2105,7 @@ theorem Spec.Iter.foldM_filterM {α β δ : Type w}
 theorem Spec.Iter.foldM_filterMap {α β γ δ : Type w}
     {n : Type w → Type w'}
     {Pred : Type w} {EPred : Type w}
-    [Iterator α Id β] [Finite α Id] [Monad n] [LawfulMonad n] [Assertion Pred] [Assertion EPred] [WPMonad n Pred EPred]
+    [Iterator α Id β] [Finite α Id] [Monad n] [LawfulMonad n] [Assertion Pred] [Assertion EPred] [∀ α, WP (n α) α Pred EPred] [WPMonad n Pred EPred]
     [IteratorLoop α Id n]
     [LawfulIteratorLoop α Id n]
     {f : β → Option γ} {g : δ → γ → n δ} {init : δ} {it : Iter (α := α) β}
@@ -2119,7 +2121,7 @@ theorem Spec.Iter.foldM_filterMap {α β γ δ : Type w}
 theorem Spec.Iter.foldM_map {α β γ δ : Type w}
     {n : Type w → Type w'}
     {Pred : Type w} {EPred : Type w}
-    [Iterator α Id β] [Finite α Id] [Monad n] [LawfulMonad n] [Assertion Pred] [Assertion EPred] [WPMonad n Pred EPred]
+    [Iterator α Id β] [Finite α Id] [Monad n] [LawfulMonad n] [Assertion Pred] [Assertion EPred] [∀ α, WP (n α) α Pred EPred] [WPMonad n Pred EPred]
     [IteratorLoop α Id n] [LawfulIteratorLoop α Id n]
     {f : β → γ} {g : δ → γ → n δ} {init : δ} {it : Iter (α := α) β}
     {P : Pred} {Q : δ → Pred} {eQ : EPred}
@@ -2132,7 +2134,7 @@ theorem Spec.Iter.foldM_map {α β γ δ : Type w}
 theorem Spec.Iter.foldM_filter {α β δ : Type w}
     {n : Type w → Type w'}
     {Pred : Type w} {EPred : Type w}
-    [Iterator α Id β] [Finite α Id] [Monad n] [LawfulMonad n] [Assertion Pred] [Assertion EPred] [WPMonad n Pred EPred]
+    [Iterator α Id β] [Finite α Id] [Monad n] [LawfulMonad n] [Assertion Pred] [Assertion EPred] [∀ α, WP (n α) α Pred EPred] [WPMonad n Pred EPred]
     [IteratorLoop α Id n] [LawfulIteratorLoop α Id n]
     {f : β → Bool} {g : δ → β → n δ} {init : δ} {it : Iter (α := α) β}
     {P : Pred} {Q : δ → Pred} {eQ : EPred}
@@ -2146,7 +2148,7 @@ theorem Spec.Iter.fold_filterMapWithPostcondition {α β γ δ : Type w}
     {n : Type w → Type w'}
     {Pred : Type w} {EPred : Type w}
     [Iterator α Id β] [Finite α Id]
-    [Monad n] [LawfulMonad n] [Assertion Pred] [Assertion EPred] [WPMonad n Pred EPred]
+    [Monad n] [LawfulMonad n] [Assertion Pred] [Assertion EPred] [∀ α, WP (n α) α Pred EPred] [WPMonad n Pred EPred]
     [IteratorLoop α Id n] [LawfulIteratorLoop α Id n]
     {f : β → PostconditionT n (Option γ)} {g : δ → γ → δ} {init : δ} {it : Iter (α := α) β}
     {P : Pred} {Q : δ → Pred} {eQ : EPred}
@@ -2162,7 +2164,7 @@ theorem Spec.Iter.fold_filterMapM {α β γ δ : Type w}
     {n : Type w → Type w'}
     {Pred : Type w} {EPred : Type w}
     [Iterator α Id β] [Finite α Id]
-    [Monad n] [MonadAttach n] [LawfulMonad n] [WeaklyLawfulMonadAttach n] [Assertion Pred] [Assertion EPred] [WPMonad n Pred EPred]
+    [Monad n] [MonadAttach n] [LawfulMonad n] [WeaklyLawfulMonadAttach n] [Assertion Pred] [Assertion EPred] [∀ α, WP (n α) α Pred EPred] [WPMonad n Pred EPred]
     [IteratorLoop α Id n] [LawfulIteratorLoop α Id n]
     {f : β → n (Option γ)} {g : δ → γ → δ} {init : δ} {it : Iter (α := α) β}
     {P : Pred} {Q : δ → Pred} {eQ : EPred}
@@ -2178,7 +2180,7 @@ theorem Spec.Iter.fold_mapWithPostcondition {α β γ δ : Type w}
     {n : Type w → Type w'}
     {Pred : Type w} {EPred : Type w}
     [Iterator α Id β] [Finite α Id]
-    [Monad n] [LawfulMonad n] [Assertion Pred] [Assertion EPred] [WPMonad n Pred EPred]
+    [Monad n] [LawfulMonad n] [Assertion Pred] [Assertion EPred] [∀ α, WP (n α) α Pred EPred] [WPMonad n Pred EPred]
     [IteratorLoop α Id n] [LawfulIteratorLoop α Id n]
     {f : β → PostconditionT n γ} {g : δ → γ → δ} {init : δ} {it : Iter (α := α) β}
     {P : Pred} {Q : δ → Pred} {eQ : EPred}
@@ -2192,7 +2194,7 @@ theorem Spec.Iter.fold_mapM {α β γ δ : Type w}
     {n : Type w → Type w'}
     {Pred : Type w} {EPred : Type w}
     [Iterator α Id β] [Finite α Id]
-    [Monad n] [MonadAttach n] [LawfulMonad n] [WeaklyLawfulMonadAttach n] [Assertion Pred] [Assertion EPred] [WPMonad n Pred EPred]
+    [Monad n] [MonadAttach n] [LawfulMonad n] [WeaklyLawfulMonadAttach n] [Assertion Pred] [Assertion EPred] [∀ α, WP (n α) α Pred EPred] [WPMonad n Pred EPred]
     [IteratorLoop α Id n] [LawfulIteratorLoop α Id n]
     {f : β → n γ} {g : δ → γ → δ} {init : δ} {it : Iter (α := α) β}
     {P : Pred} {Q : δ → Pred} {eQ : EPred}
@@ -2206,7 +2208,7 @@ theorem Spec.Iter.fold_filterWithPostcondition {α β δ : Type w}
     {n : Type w → Type w'}
     {Pred : Type w} {EPred : Type w}
     [Iterator α Id β] [Finite α Id]
-    [Monad n] [LawfulMonad n] [Assertion Pred] [Assertion EPred] [WPMonad n Pred EPred]
+    [Monad n] [LawfulMonad n] [Assertion Pred] [Assertion EPred] [∀ α, WP (n α) α Pred EPred] [WPMonad n Pred EPred]
     [IteratorLoop α Id n] [LawfulIteratorLoop α Id n]
     {f : β → PostconditionT n (ULift Bool)} {g : δ → β → δ} {init : δ} {it : Iter (α := α) β}
     {P : Pred} {Q : δ → Pred} {eQ : EPred}
@@ -2220,7 +2222,7 @@ theorem Spec.Iter.fold_filterM {α β δ : Type w}
     {n : Type w → Type w'}
     {Pred : Type w} {EPred : Type w}
     [Iterator α Id β] [Finite α Id]
-    [Monad n] [MonadAttach n] [LawfulMonad n] [WeaklyLawfulMonadAttach n] [Assertion Pred] [Assertion EPred] [WPMonad n Pred EPred]
+    [Monad n] [MonadAttach n] [LawfulMonad n] [WeaklyLawfulMonadAttach n] [Assertion Pred] [Assertion EPred] [∀ α, WP (n α) α Pred EPred] [WPMonad n Pred EPred]
     [IteratorLoop α Id n] [LawfulIteratorLoop α Id n]
     {f : β → n (ULift Bool)} {g : δ → β → δ} {init : δ} {it : Iter (α := α) β}
     {P : Pred} {Q : δ → Pred} {eQ : EPred}
@@ -2311,7 +2313,7 @@ noncomputable abbrev StringInvariant.withEarlyReturnNewDo {s : String} {β : Typ
       ⊔ (iSup fun r => ⌜x = some r ∧ pos = s.endPos⌝ ⊓ onReturn r b)
 
 @[spec]
-theorem Spec.forIn_string
+theorem Spec.forIn_string [LawfulMonad m]
     {s : String} {init : β} {f : Char → β → m (ForInStep β)}
     (inv : StringInvariant s β Pred)
     {epost : EPred}
@@ -2368,7 +2370,7 @@ noncomputable abbrev StringSliceInvariant.withEarlyReturnNewDo {s : String.Slice
       ⊔ (iSup fun r => ⌜x = some r ∧ pos = s.endPos⌝ ⊓ onReturn r b)
 
 @[spec]
-theorem Spec.forIn_stringSlice
+theorem Spec.forIn_stringSlice [LawfulMonad m]
     {s : String.Slice} {init : β} {f : Char → β → m (ForInStep β)}
     (inv : StringSliceInvariant s β Pred)
     {epost : EPred}
@@ -2410,7 +2412,7 @@ universe u
 
 variable {α β : Type u} {m : Type u → Type v} {Pred : Type u} {EPred : Type u}
 variable [Monad m] [Lean.Order.MonadTail m] [Assertion Pred] [Assertion EPred]
-  [WPMonad m Pred EPred]
+  [∀ α, WP (m α) α Pred EPred] [WPMonad m Pred EPred]
 
 /--
 An invariant for a `whileM` loop, given as a predicate over the `α ⊕ β` cursor:
